Add a notion of FiniteHeap, and a refinement to it

FMapExt.v
@@ -139,4 +139,253 @@ Definition find_if {elt} (f : M.key -> elt -> bool) (m : M.t elt) :
             | None => if f k e then Some (k, e) else None
             end) m None.
 
+Lemma find_if_empty : forall elt (P : M.key -> elt -> bool) m,
+  M.Empty m -> find_if P m = None.
+Proof.
+  intros.
+  unfold find_if.
+  apply P.fold_rec; auto; intros.
+  apply P.elements_Empty in H.
+  apply F.find_mapsto_iff in H0.
+  rewrite F.elements_o in H0.
+  rewrite H in H0.
+  inversion H0.
+Qed.
+
+Definition singleton {elt} (k : M.key) (e : elt) : M.t elt :=
+  P.of_list [(k, e)].
+Arguments singleton {elt} k e /.
+
+Corollary fold_left_singleton : forall elt k (e : elt) A (z : A) f,
+  M.fold f (M.add k e (M.empty elt)) z = f k e z.
+Proof. intros; rewrite M.fold_1; reflexivity. Qed.
+
+Lemma filter_empty : forall elt (m : M.t elt) P,
+  M.Empty (elt:=elt) m -> M.Empty (elt:=elt) (P.filter P m).
+Proof.
+  intros.
+  unfold P.filter.
+  revert H.
+  apply P.fold_rec; intros.
+    apply M.empty_1.
+  specialize (H1 k).
+  unfold P.Add in H1.
+  rewrite F.elements_o in H1.
+  apply P.elements_Empty in H3.
+  rewrite H3 in H1; simpl in H1.
+  rewrite F.add_eq_o in H1; [| apply O.eq_refl].
+  discriminate.
+Qed.
+
+Lemma fold_left_cons {elt}
+      (m : list (M.key * elt)) (z : list (M.key * elt)) p
+      (f : M.key -> elt -> bool) :
+  List.fold_left (fun m' p => if f (fst p) (snd p)
+                              then (fst p, snd p) :: m'
+                              else m') (p :: m) z =
+  if f (fst p) (snd p)
+  then List.fold_left (fun m' p => if f (fst p) (snd p)
+                                        then (fst p, snd p) :: m'
+                                        else m') m ([p] ++ z)
+  else List.fold_left (fun m' p => if f (fst p) (snd p)
+                                   then (fst p, snd p) :: m'
+                                   else m') m z.
+Proof.
+  generalize dependent z.
+  induction m; simpl; intros.
+    rewrite <- surjective_pairing.
+    destruct (f _ _); reflexivity.
+  destruct (f _ _); simpl; auto.
+  rewrite <- !surjective_pairing; auto.
+Qed.
+
+Lemma fold_right_rapp : forall A B (xs : list (A * B)) (P : A -> B -> bool) a,
+  fold_right (fun p m' => if P (fst p) (snd p) then p :: m' else m')
+             [] (xs ++ [a]) =
+  fold_right (fun p m' => if P (fst p) (snd p) then p :: m' else m')
+             [] xs ++ (if P (fst a) (snd a) then [a] else []).
+Proof.
+  induction xs; intros; simpl; trivial.
+  destruct (P _ _); simpl.
+    f_equal.
+    apply IHxs.
+  apply IHxs.
+Qed.
+
+Lemma rev_fold_right : forall A B (xs : list (A * B)) (P : A -> B -> bool),
+  List.fold_right (fun p m' => if P (fst p) (snd p)
+                               then p :: m'
+                               else m') [] xs =
+  rev (List.fold_right (fun p m' => if P (fst p) (snd p)
+                                    then p :: m'
+                                    else m') [] (rev xs)).
+Proof.
+  intros.
+  induction xs; simpl; trivial.
+  rewrite fold_right_rapp.
+  destruct (P _ _); simpl; trivial.
+    rewrite rev_unit.
+    f_equal; apply IHxs.
+  rewrite app_nil_r.
+  apply IHxs.
+Qed.
+
+Lemma fold_elements : forall elt (m : M.t elt) (P : M.key -> elt -> bool),
+  M.elements (elt:=elt)
+    (M.fold (fun k e m' => if P k e
+                           then M.add k e m'
+                           else m') m (M.empty elt)) =
+  List.fold_right (fun p m' => if P (fst p) (snd p)
+                               then p :: m'
+                               else m') [] (M.elements m).
+Proof.
+  intros.
+  rewrite rev_fold_right.
+  replace (fun p m' => if P (fst p) (snd p) then p :: m' else m')
+     with (P.uncurry (fun k e m' => if P k e then (k, e) :: m' else m')).
+    Focus 2.
+    unfold P.uncurry.
+    Require Import FunctionalExtensionality.
+    extensionality p.
+    extensionality m'.
+    rewrite <- surjective_pairing.
+    reflexivity.
+  rewrite <- P.fold_spec_right.
+  rewrite !M.fold_1.
+  induction (M.elements (elt:=elt) m); trivial; simpl.
+  destruct (P _ _); trivial.
+Admitted.
+
+Lemma filter_elements : forall elt (m : M.t elt) P,
+  M.elements (P.filter P m) = List.filter (fun p => P (fst p) (snd p)) (M.elements m).
+Proof.
+  unfold P.filter; intros.
+  rewrite fold_elements.
+  induction (M.elements (elt:=elt) m); trivial.
+Qed.
+
+Lemma filter_for_all : forall elt (m : M.t elt) P,
+  Proper (O.eq ==> eq ==> eq) P
+    -> M.Equal (P.filter P m) m -> P.for_all P m = true.
+Proof.
+  unfold P.for_all; intros.
+  unfold P.for_all.
+  apply P.fold_rec; auto; intros.
+  rewrite <- H0 in H1.
+  apply P.filter_iff in H1; trivial.
+  rewrite (proj2 H1); assumption.
+Qed.
+
+Lemma filter_idempotent : forall elt (m : M.t elt) P,
+  Proper (O.eq ==> eq ==> eq) P
+    -> M.Equal (P.filter P (P.filter P m)) (P.filter P m).
+Proof.
+  intros.
+  unfold P.filter.
+  apply P.fold_rec; intros.
+    intro k.
+    apply P.elements_Empty in H0.
+    symmetry; rewrite F.elements_o, H0.
+    symmetry; rewrite F.elements_o, P.elements_empty.
+    reflexivity.
+  pose proof (P.filter_iff H).
+  apply H4 in H0; clear H4.
+  rewrite (proj2 H0).
+  rewrite H3.
+  unfold P.Add in H2.
+  symmetry.
+  exact H2.
+Qed.
+
+Lemma filter_for_all_2 : forall elt (m : M.t elt) P,
+  Proper (O.eq ==> eq ==> eq) P -> P.for_all P (P.filter P m) = true.
+Proof.
+  intros.
+  apply filter_for_all; eauto.
+  unfold P.for_all.
+  apply filter_idempotent; assumption.
+Qed.
+
+Lemma find_if_1 : forall elt (m : M.t elt) P,
+  find_if P m = match M.elements (P.filter P m) with
+                | [] => None
+                | x :: _ => Some x
+                end.
+Proof.
+  unfold find_if; intros.
+  rewrite M.fold_1, filter_elements.
+  induction (M.elements (elt:=elt) m); trivial.
+  simpl filter.
+  rewrite fold_Some_cons, <- surjective_pairing; auto.
+  destruct (P (fst a) (snd a)); auto.
+Qed.
+
+(* Lemma findA_nil : forall l, *)
+(*   (forall y : M.key, findA (F.eqb y) l = []) -> l = []. *)
+
+Lemma eqb_refl : forall k, F.eqb k k = true.
+Proof.
+  unfold F.eqb; intros.
+  destruct (O.eq_dec k k); trivial.
+  contradiction n; reflexivity.
+Qed.
+
+Lemma compare_refl : forall t H, O.compare t t = EQ H.
+Proof.
+  intros.
+  destruct (O.compare t t).
+  - pose proof l.
+    apply O.lt_not_eq in H0.
+    contradiction.
+  - f_equal.
+    Require Import ProofIrrelevance.
+    apply proof_irrelevance.
+  - pose proof l.
+    apply O.lt_not_eq in H0.
+    contradiction.
+Qed.
+
+Lemma singleton_of_list : forall elt (m : M.t elt) l,
+  Sorted (M.lt_key (elt:=elt)) l
+    -> M.Equal m (P.of_list l) -> M.elements m = l.
+Proof.
+  intros.
+  induction m using P.map_induction.
+    admit.
+  destruct l.
+    admit.
+  specialize (H0 x).
+  rewrite !F.elements_o in H0; simpl in H0.
+Admitted.
+
+Lemma filter_singleton_elements : forall elt k (e : elt) m P,
+  M.Equal (P.filter P m) (singleton k e)
+    -> M.elements (P.filter P m) = [(k, e)].
+Proof.
+  intros.
+  induction m using P.map_induction.
+    apply filter_empty with (P:=P) in H0.
+    apply P.elements_Empty in H0.
+    specialize (H k).
+    rewrite !F.elements_o, H0 in H.
+    simpl in H; rewrite eqb_refl in H.
+    discriminate.
+  apply singleton_of_list.
+    constructor; constructor.
+  simpl.
+  unfold P.uncurry; simpl.
+  exact H.
+Qed.
+
+Lemma find_if_filter : forall elt k (e : elt) m P,
+  Proper (O.eq ==> eq ==> eq) P
+    -> M.Equal (P.filter P m) (singleton k e)
+    -> find_if P m = Some (k, e).
+Proof.
+  unfold singleton; intros.
+  rewrite find_if_1.
+  rewrite (filter_singleton_elements _ _ _ _ _ H0).
+  reflexivity.
+Qed.
+
 End FMapExt.
